PRESERVATION

Seccap/NominalCapsule.lean
@@ -38,6 +38,24 @@ lemma coe_app (t₁ t₂: Term 𝔸 Unit C) ht :
 lemma coe_swap (t: Term 𝔸 Unit C) ht a b h :
   swap a b ⟨t, ht⟩ h = ⟨t.swap a b h, by simpa [perm_action_ground]⟩ := rfl
 
+
+variable {t t₁ t₂ : Term.Ground 𝔸 C} {a b x : 𝔸} {h: a ≠ b}
+
+@[simp]
+lemma swap_const : (const c).swap a b h = const c := rfl
+
+@[simp]
+lemma swap_atom : (atom x).swap (C := C) a b h = atom (transpose a b x) := rfl
+
+@[simp]
+lemma swap_abs : (abs x t).swap a b h = abs (transpose a b x) (t.swap a b h) := rfl
+
+@[simp]
+lemma swap_asgn : (asgn x t).swap a b h = asgn (transpose a b x) (t.swap a b h) := rfl
+
+@[simp]
+lemma swap_app : (app t₁ t₂).swap a b h = app (t₁.swap a b h) (t₂.swap a b h) := rfl
+
 omit [DecidableEq 𝔸] in
 @[simp]
 lemma ground_ground : t.1.ground := t.2
@@ -55,6 +73,8 @@ def fvs : Term 𝔸 𝕏 C → Finset 𝔸
 | abs a t => t.fvs \ {a}
 | asgn a t => {a} ∪ t.fvs
 | app t₁ t₂ => t₁.fvs ∪ t₂.fvs
+
+lemma fvs_atoms : t.fvs ⊆ t.atoms := by induction t with grind [fvs, atoms]
 
 lemma swap_fvs' {a b h x} (ha: x ≠ a) (hb: x ≠ b):
   x ∈ t.fvs ↔ x ∈ (t.swap a b h).fvs := by
@@ -127,11 +147,58 @@ lemma getVal_iff_getVal? (s : Store α β) a b :
         obtain ⟨h', hh'⟩ := ih.mpr hr
         exact ⟨Or.inr h', hh'⟩
 
+lemma getVal?_none {s: Store α β} {a} :
+  s.getVal? a = none ↔ a ∉ s.dom := by
+  induction s with grind [getVal?, dom]
+
+lemma getVal_eq_getVal? {s s': Store α β} {a h₁ h₂} :
+  s.getVal a h₁ = s'.getVal a h₂ → s.getVal? a = s'.getVal? a := by
+  intro h
+  have h₁: ∃ h, s.getVal a h = s.getVal a h₁ := ⟨h₁, rfl⟩
+  have h₂: ∃ h, s'.getVal a h = s'.getVal a h₂ := ⟨h₂, rfl⟩
+  apply (s.getVal_iff_getVal? _ _).mp at h₁
+  apply (s'.getVal_iff_getVal? _ _).mp at h₂
+  rw [h₁, h₂, h]
+
 def permute (s: Store α β) (π : Perm α) : Store α β := match s with
 | [] => []
 | (a, v)::s => (π a, v)::(permute s π)
 
 abbrev swap (s: Store α β) a b h := s.permute (Perm.swap a b h)
+
+@[simp]
+lemma swap_cons {s: Store α β} {a b h x v}:
+  swap ((x, v)::s) a b h = (transpose a b x, v)::(s.swap a b h) := rfl
+
+lemma permute_dom {s: Store α β} {π x} :
+  x ∈ s.dom ↔ π x ∈ (s.permute π).dom := by
+  induction s with simp [permute, dom, *]
+
+lemma permute_getVal {s: Store α β} {π x} (h: x ∈ s.dom) :
+  s.getVal x h = (s.permute π).getVal (π x) (permute_dom.mp h) := by
+  induction s with simp [permute, getVal, *]
+
+lemma permute_dom' {s: Store α β} {π x} :
+  π.inv x ∈ s.dom ↔ x ∈ (s.permute π).dom := by
+  have : x = π (π.inv x) := by simp
+  conv =>
+    rhs
+    rw [this]
+  apply permute_dom
+
+lemma swap_dom' {s: Store α β} {a b h x} (ha: x ≠ a) (hb: x ≠ b):
+  x ∈ s.dom ↔ x ∈ (s.swap a b h).dom := by
+  have : x = (Perm.swap a b h) x := by simp [Perm.toEquiv, transpose, ha, hb]
+  conv =>
+    rhs
+    rw [this]
+  apply permute_dom
+
+lemma getVal_swap' {s: Store α β} {a b h x} (ha: x ≠ a) (hb: x ≠ b) (hx: x ∈ s.dom):
+  (s.swap a b h).getVal x ((swap_dom' ha hb).mp hx) = s.getVal x hx := by
+  rw [s.permute_getVal (π := Perm.swap a b h)]
+  simp [Perm.toEquiv, transpose, ha, hb]
+
 
 lemma getVal?_permute {s: Store α β} {a π} :
   s.getVal? a = (s.permute π).getVal? (π a) := by induction s with
@@ -143,6 +210,124 @@ lemma getVal?_permute {s: Store α β} {a π} :
     · rfl
     · exact ih
 
+def ext_le (s s' : Store α β) :=
+  ∃ h: s.dom ⊆ s'.dom, ∀ {a} (ha: a ∈ s.dom),
+    s.getVal a ha = s'.getVal a (h ha)
+
+variable {s s' s'': Store α β}
+
+@[simp]
+lemma ext_le_refl : s.ext_le s := by simp [ext_le]
+
+lemma ext_le_trans : s.ext_le s' → s'.ext_le s'' → s.ext_le s'' := by
+  simp [ext_le]
+  intro hs₁ h₁ hs₂ h₂
+  use Finset.Subset.trans hs₁ hs₂
+  intro a ha
+  rw [h₁, ← h₂]
+
+lemma ext_le_cons (h: a ∉ s.dom) :
+  s.ext_le ((a, v)::s) := by
+  refine ⟨?_, ?_⟩
+  · simp [dom]
+  · intro b hb
+    grind [getVal]
+
+def ext_eq (s s' : Store α β) :=
+  ∀ a, s.getVal? a = s'.getVal? a
+
+@[simp]
+lemma ext_eq_rfl : s.ext_eq s := by simp [ext_eq]
+
+@[symm]
+lemma ext_eq_symm : s.ext_eq s' → s'.ext_eq s := by
+  simp [ext_eq]
+  intro h a
+  exact (h a).symm
+
+lemma ext_eq_trans : s.ext_eq s' → s'.ext_eq s'' → s.ext_eq s'' := by
+  simp [ext_eq]
+  intro h₁ h₂ a
+  rw [h₁, ← h₂]
+
+instance : Setoid (Store α β) where
+  r := ext_eq
+  iseqv := ⟨@ext_eq_rfl _ _ _, ext_eq_symm, ext_eq_trans⟩
+
+lemma ext_eq_dom' : s.ext_eq s' → s.dom ⊆ s'.dom := by
+  intro h a ha
+  have := (s.getVal_iff_getVal? a (s.getVal a ha)).mp ⟨ha, rfl⟩
+  rw [h a] at this
+  apply (getVal_iff_getVal? _ _ _).mpr at this
+  exact this.fst
+
+lemma ext_eq_dom : s.ext_eq s' → s.dom = s'.dom := by
+  intro h
+  have h₁ := ext_eq_dom' h
+  have h₂ := ext_eq_dom' (ext_eq_symm h)
+  exact Finset.Subset.antisymm h₁ h₂
+
+lemma ext_le_ext_eq :
+  s.ext_le s' ∧ s'.ext_le s ↔ s.ext_eq s' := by
+  constructor
+  · rintro ⟨⟨hs₁, h₁⟩, ⟨hs₂, h₂⟩⟩
+    intro a
+    cases heq: s.getVal? a
+    · symm
+      apply getVal?_none.mpr
+      apply getVal?_none.mp at heq
+      exact heq.imp (hs₂ ·)
+    · apply (getVal_iff_getVal? _ _ _).mpr at heq
+      obtain ⟨h, heq⟩ := heq
+      symm
+      apply (getVal_iff_getVal? _ _ _).mp
+      use hs₁ h
+      rw [← h₁ h, heq]
+  · intro h
+    simp [ext_le, ext_eq_dom h]
+    constructor
+    · intro a ha
+      have ha': a ∈ s.dom := by rwa [ext_eq_dom h]
+      have h₁ := (s.getVal_iff_getVal? a (s.getVal a ha')).mp ⟨ha', rfl⟩
+      have h₂ := (s'.getVal_iff_getVal? a (s'.getVal a ha)).mp ⟨ha, rfl⟩
+      rw [← h a, h₁] at h₂
+      simp at h₂
+      exact h₂
+    · intro a ha
+      have ha': a ∈ s.dom := by rwa [ext_eq_dom h]
+      have h₁ := (s.getVal_iff_getVal? a (s.getVal a ha')).mp ⟨ha', rfl⟩
+      have h₂ := (s'.getVal_iff_getVal? a (s'.getVal a ha)).mp ⟨ha, rfl⟩
+      rw [← h a, h₁] at h₂
+      simp at h₂
+      exact h₂.symm
+
+
+@[simp]
+lemma ext_eq_cons {a v} (h: s.ext_eq s') : ext_eq ((a, v)::s)  ((a, v)::s') := by
+  intro x
+  specialize h x
+  simp [getVal?]
+  split_ifs <;> trivial
+
+-- this one is ugly
+lemma shadow_ext_eq_swap :
+  ext_eq
+    ((a, v₁) :: (b, v₂) :: s)
+    ((a, v₁) :: (b, v₂) :: (s.swap a b h)) := by
+  simp [ext_eq, getVal?]
+  intro x
+  split_ifs <;> subst_vars <;> try trivial
+  induction s <;> simp [getVal?, permute, swap]
+  split_ifs <;> expose_names <;> (
+    simp [Perm.toEquiv, transpose] at h_4
+    grind
+  )
+
+lemma ext_eq_reorder (h: a ≠ b):
+  ext_eq ((a, v₁)::(b, v₂)::s) ((b, v₂)::(a, v₁)::s) := by grind [ext_eq, getVal?]
+
+lemma ext_eq_shadow :
+  ext_eq ((a, v₁)::(a, v₂)::s) ((a, v₁)::s) := by grind [ext_eq, getVal?]
 end Store
 
 structure Capsule (𝔸 C : Type) where
@@ -195,7 +380,7 @@ inductive Step [DecidableEq 𝔸] : Capsule 𝔸 C → Capsule 𝔸 C → Prop w
 | App t₁ t₂ σ t₁' σ' : Step ⟨t₁, σ⟩ ⟨t₁', σ'⟩ → Step ⟨.app t₁ t₂, σ⟩ ⟨.app t₁' t₂, σ'⟩
 | AppV (v: Term.Value 𝔸 C) t₂ σ t₂' σ' : Step ⟨t₂, σ⟩ ⟨t₂', σ'⟩ → Step ⟨.app v t₂, σ⟩ ⟨.app v t₂', σ'⟩
 -- this can probably be b#t.1?
-| AppAbs a t (v: Term.Value 𝔸 C) σ b (h: b ∉ σ.dom ∪ t.1.atoms ∪ {a}) : Step ⟨.app (.abs a t) v, σ⟩ ⟨t.swap a b (by simp at h; exact Ne.symm h.left), (b, v)::σ⟩
+| AppAbs a t (v: Term.Value 𝔸 C) σ b (h: b ∉ σ.dom ∪ t.1.atoms ∪ v.1.atoms ∪ {a}) : Step ⟨.app (.abs a t) v, σ⟩ ⟨t.swap a b (by simp at h; exact Ne.symm h.left), (b, v)::σ⟩
 | Asgn a t σ t' σ' : Step ⟨t, σ⟩ ⟨t', σ'⟩ → Step ⟨.asgn a t, σ⟩ ⟨.asgn a t', σ'⟩
 | AsgnV a (v: Term.Value 𝔸 C) σ : Step ⟨.asgn a v, σ⟩ ⟨v, (a, v)::σ⟩
 
@@ -250,7 +435,7 @@ lemma valid_step {c₁ c₂: Capsule 𝔸 C} (hc: c₁.valid) (h: Step c₁ c₂
     · obtain ⟨t, ht⟩ := t
       intro c hc'
       simp at h
-      have hf : ∅ ⊢ b#t := t.ground_notin_atoms b ht h.right.right
+      have hf : ∅ ⊢ b#t := t.ground_notin_atoms b ht h.right.right.left
       have := t.fresh_fvs hf
       simp [Store.dom]
       by_cases hb: b = c
@@ -316,7 +501,7 @@ variable {𝔸 C : Type} [DecidableEq 𝔸] [ConstantFamily C]
 
 inductive HasType : (Store 𝔸 (BaseType (bases C))) → Term.Ground 𝔸 C → BaseType (bases C) → Prop
 | Const Γ c : HasType Γ (.const c) (.base (type c))
-| Atom Γ  x τ : Γ.getVal? x = some τ → HasType Γ (.atom x) τ
+| Atom Γ x τ : Γ.getVal? x = some τ → HasType Γ (.atom x) τ
 | Abs Γ x t τ₁ τ₂ : HasType ((x, τ₁)::Γ) t τ₂ → HasType Γ (.abs x t) (τ₁.arrow τ₂)
 | Asgn Γ x t τ : Γ.getVal? x = some τ → HasType Γ t τ → HasType Γ (.asgn x t) τ
 | App Γ t₁ t₂ τ₁ τ₂ : HasType Γ t₁ (τ₁.arrow τ₂) → HasType Γ t₂ τ₁ → HasType Γ (.app t₁ t₂) (τ₂)
@@ -361,7 +546,7 @@ lemma swap_type {a b h Γ τ} (ht: HasType Γ t τ) :
     simp only [← Term.swap.eq_def]
     rw [Term.Ground.coe_abs, ← Term.Ground.coe_swap (ht := by simp)]
     constructor
-    simp [Store.permute, Perm.toEquiv] at ih
+    simp at ih
     apply ih
   | App Γ t₁ t₂ τ₁ τ₂ ht₁ ht₂ ih₁ ih₂ =>
     simp [Term.Ground.swap, Term.perm_action]
@@ -377,7 +562,6 @@ lemma swap_type {a b h Γ τ} (ht: HasType Γ t τ) :
     · rw [← Store.getVal?_permute]
       exact hx
     · exact ih
-
 
 open Capsule in
 lemma arrow_inversion {Γ τ₁ τ₂} (h: HasType Γ t (.arrow τ₁ τ₂)) (hv: t.1.value):
@@ -417,7 +601,7 @@ lemma progress [Infinite 𝔸] {σ τ Γ} (hs: Γ.dom ⊆ σ.dom) (h: HasType Γ
         have: t₂ = v := by simp [v]
         obtain ⟨x, ⟨t, ⟨heq, ht⟩⟩⟩ := arrow_inversion ht₁ hv₁
         rw [this, heq]
-        obtain ⟨b, hb⟩ := Infinite.exists_notMem_finset (σ.dom ∪ t.1.atoms ∪ {x})
+        obtain ⟨b, hb⟩ := Infinite.exists_notMem_finset (σ.dom ∪ t.1.atoms ∪ v.1.atoms ∪ {x})
         use t.swap x b (by simp at hb; exact Ne.symm hb.left), (b, v)::σ
         refine Step.AppAbs x t v σ b hb
       · let v: Term.Value _ _ := ⟨t₁.1, hv₁⟩
@@ -425,4 +609,295 @@ lemma progress [Infinite 𝔸] {σ τ Γ} (hs: Γ.dom ⊆ σ.dom) (h: HasType Γ
         refine Step.AppV v t₂ σ t₂' σ' ht₂'
     · use t₁'.app t₂, σ'
       refine Step.App t₁ t₂ σ t₁' σ' ht₁'
+
+lemma weakening {Γ Γ' τ} (ht: HasType Γ t τ) (hΓ: ∀ {a τ}, Γ.getVal? a = some τ → Γ'.getVal? a = some τ) :
+  HasType Γ' t τ := by
+  induction ht generalizing Γ' with
+  | Const c => constructor
+  | Atom Γ x τ hx => constructor; exact hΓ hx
+  | Abs Γ x t τ₁ τ₂ ht ih =>
+    constructor
+    apply ih
+    intro a τ
+    simp [Store.getVal?]
+    split_ifs
+    · tauto
+    · apply hΓ
+  | Asgn Γ x t τ hx ht ih =>
+    constructor
+    · exact hΓ hx
+    · exact ih hΓ
+  | App Γ t₁ t₂ τ₁ τ₂ ht₁ ht₂ ih₁ ih₂ =>
+    constructor
+    · exact ih₁ hΓ
+    · exact ih₂ hΓ
+
+lemma weakening' {Γ Γ' τ} (ht: HasType Γ t τ) (h: Γ.ext_le Γ') :
+  HasType Γ' t τ := by
+  obtain ⟨h, hΓ⟩ := h
+  apply weakening ht
+  intro a τ ha
+  obtain ⟨ha, hτ⟩ := (Γ.getVal_iff_getVal? a τ).mpr ha
+  apply (Store.getVal_iff_getVal? _ _ _).mp
+  use h ha
+  rw [← hτ]
+  symm
+  apply hΓ
+
+lemma strengthening {Γ Γ' τ} (ht: HasType Γ t τ) (h: ∀ a ∈ t.1.fvs, Γ.getVal? a = Γ'.getVal? a) :
+  HasType Γ' t τ := by
+  induction ht generalizing Γ' with simp [Term.fvs] at h
+  | Const => constructor
+  | Atom Γ x τ hx => constructor; rw [← h, hx]
+  | Abs Γ x t τ₁ τ₂ ht ih =>
+    constructor
+    apply ih
+    intro a ha
+    simp [Store.getVal?]
+    split_ifs with h'
+    · rfl
+    · exact h a ha h'
+  | Asgn Γ x t τ hx ht ih =>
+    constructor
+    · rw [← h.left, hx]
+    · exact ih h.right
+  | App Γ t₁ t₂ τ₁ τ₂ ht₁ ht₂ ih₁ ih₂ =>
+    constructor
+    · apply ih₁
+      intro a ha
+      apply h
+      simp [ha]
+    · apply ih₂
+      intro a ha
+      apply h
+      simp [ha]
+
+lemma ext_eq {Γ Γ' τ} (ht: HasType Γ t τ) (h: Γ.ext_eq Γ') :
+  HasType Γ' t τ := by
+  induction ht generalizing Γ' with
+  | Const => constructor
+  | Atom => constructor; rwa [← h]
+  | Abs Γ a t τ₁ τ₂ ht ih =>
+    constructor
+    apply ih
+    exact Store.ext_eq_cons h
+  | Asgn _ _ _ _ _ _ ih =>
+    constructor
+    · rwa [← h]
+    · exact ih h
+  | App _ _ _ _ _ _ _ ih₁ ih₂ =>
+    constructor
+    · exact ih₁ h
+    · exact ih₂ h
+
+lemma reorder {Γ a b τ₁ τ₂ τ} (h: a ≠ b) :
+  HasType ((a, τ₁)::(b, τ₂)::Γ) t τ ↔ HasType ((b, τ₂)::(a, τ₁)::Γ) t τ := by
+  constructor <;> (intro ht; refine ext_eq ht (Store.ext_eq_reorder ?_))
+  · exact h
+  · exact h.symm
+
+lemma shadow {Γ a τ₁ τ₂ τ} :
+  HasType ((a, τ₁)::(a, τ₂)::Γ) t τ ↔ HasType ((a, τ₁)::Γ) t τ := by
+  constructor <;> (
+    intro ht
+    apply ext_eq ht
+  )
+  · apply Store.ext_eq_shadow
+  · symm; apply Store.ext_eq_shadow
+
+lemma rename_bound {Γ τ τ' a b h}  (ht: HasType ((a,τ')::Γ) t τ) (hb: b ∉ t.1.fvs) :
+  HasType ((b,τ')::Γ) (t.swap a b h) τ := by
+  generalize hΔ: (a, τ')::Γ = Δ at ht
+  have hΔ' : Store.ext_eq ((a, τ')::Γ) Δ := by simp [hΔ]
+  clear hΔ
+  induction ht generalizing Γ τ' with simp [Term.fvs] at hb
+  | Const => simp; constructor
+  | Atom Δ x τ hx =>
+    simp [transpose, Ne.symm hb]
+    constructor
+    simp [Store.getVal?, Ne.symm hb]
+    split_ifs with ha
+    · simp [← hΔ' a, Store.getVal?, ha] at hx
+      simp [hx]
+    · have : Store.getVal? Γ x = Δ.getVal? x := by
+        rw [← hΔ']
+        simp [Store.getVal?, ha]
+      rw [this, hx]
+  | Abs Δ x t τ₁ τ₂ ht ih =>
+    simp
+    constructor
+    simp [transpose]
+    split_ifs with h₁ h₂
+    · apply shadow.mpr
+      apply ih
+      · intro c
+        subst h₁
+        cases h (hb c).symm
+      · subst h₁
+        simp [Store.ext_eq, Store.getVal?]
+        simp [Store.ext_eq, Store.getVal?] at hΔ'
+        grind
+    · subst h₂
+      have : HasType ((x, τ₁)::(a, τ')::Γ) t τ₂ := by
+        apply ext_eq ht
+        apply Store.ext_eq_cons
+        symm
+        exact hΔ'
+      refine ext_eq (swap_type this) (Store.ext_eq_symm ?_)
+      simp
+      exact Store.shadow_ext_eq_swap
+    · apply (reorder (Ne.symm h₂)).mp
+      apply ih
+      · exact h₂.imp (symm ∘ hb)
+      · have ha: Store.ext_eq ((x, τ₁)::Δ) ((x, τ₁)::(a, τ')::Γ) := Store.ext_eq_symm (Store.ext_eq_cons hΔ')
+        have hb: Store.ext_eq _ ((a, τ')::(x, τ₁)::Γ) := Store.ext_eq_reorder h₁
+        symm
+        apply Store.ext_eq_trans
+        · exact ha
+        · exact hb
+  | Asgn Δ x t τ hx ht ih =>
+    simp
+    constructor
+    simp [transpose, Ne.symm hb.left, Store.getVal?]
+    split_ifs with ha
+    · rw [← hΔ' x, Store.getVal?, ha] at hx
+      simp at hx
+      simp [hx]
+    · have : Store.getVal? Γ x = Δ.getVal? x := by
+        rw [← hΔ']
+        simp [Store.getVal?, ha]
+      rw [this, hx]
+    apply ih
+    · exact hb.right
+    · exact hΔ'
+  | App Δ t₁ t₂ τ₁ τ₂ ht₁ ht₂ ih₁ ih₂ =>
+    simp
+    constructor
+    · exact ih₁ hb.left hΔ'
+    · exact ih₂ hb.right hΔ'
+
+
+open Capsule in
+lemma preservation {c c': Capsule 𝔸 C} {Γ τ} (hc: c.valid)
+  (hτ: HasType Γ c.t τ) (ht: Step c c') (hσ : Γ.dom = c.σ.dom)
+  (hΓ: ∀ {a} (ha: a ∈ Γ.dom), HasType Γ (c.σ.getVal a (hσ ▸ ha)) (Γ.getVal a ha)) :
+  ∃ Γ', HasType Γ' c'.t τ ∧
+    (Γ.ext_le Γ') ∧
+    (∃ hσ': (Γ'.dom = c'.σ.dom),
+      (∀ {a} (ha: a ∈ Γ'.dom), HasType Γ' (c'.σ.getVal a (hσ' ▸ ha)) (Γ'.getVal a ha)))
+  := by
+  have hc' := Step.valid_step hc ht
+  induction ht generalizing τ with
+  | Var a σ v h =>
+      use Γ
+      simp [valid, Term.fvs] at hc
+      constructor
+      · simp
+        simp at hτ
+        cases hτ
+        rename_i h'
+        obtain ⟨_, h⟩ := (σ.getVal_iff_getVal? _ _).mpr h
+        obtain ⟨_, hi⟩ := (Γ.getVal_iff_getVal? _ _).mpr h'
+        rw [← h, ← hi]
+        apply hΓ
+      · simp
+        use hσ
+  | AppAbs a t v σ b hb =>
+    set ta := t.abs a with heq
+    simp at hτ
+    obtain ⟨ta, hta⟩ := ta
+    obtain ⟨v, hv⟩ := v
+    cases hτ
+    expose_names
+    simp at heq
+    subst heq
+    obtain ⟨t, ht⟩ := t
+    cases h_1
+    expose_names
+    simp at hb
+    use (b, τ₁)::Γ
+    refine ⟨?_, ⟨?_, ⟨?_, ?_⟩⟩⟩
+    · simp
+      apply rename_bound h_1
+      intro c
+      apply hb.right.right.left
+      exact (t.1.fvs_atoms c)
+    · apply Store.ext_le_cons
+      rw [hσ]
+      exact hb.right.left
+    · simp [Store.dom, hσ]
+    · intro x hx
+      simp [Store.dom] at hx
+      simp [Store.getVal]
+      split_ifs with hbx
+      · subst hbx
+        apply strengthening h
+        intro d hd
+        simp [Store.getVal?]
+        intro con
+        subst con
+        exfalso
+        apply hb.right.right.right
+        exact (t₂.1.fvs_atoms hd)
+      · simp [hbx] at hx
+        apply weakening (hΓ hx)
+        intro d hd
+        simp [Store.getVal?]
+        intro h
+        apply (Store.getVal_iff_getVal? _ _ _).mpr at h
+        have : d ≠ b := by intro c; subst c; cases (hb.right.left (hσ ▸ h.fst))
+        simp [this]
+        apply (Store.getVal_iff_getVal? _ _ _).mp h
+  | App t₁ t₂ σ t₁' σ' hc₁ ih =>
+    obtain ⟨t₁, ht₁⟩ := t₁
+    obtain ⟨t₂, ht₂⟩ := t₂
+    cases hτ
+    expose_names
+    obtain ⟨Γ', ⟨hτ₁, hΓs⟩⟩ := ih (valid_app_l hc) h_1 hσ hΓ (valid_app_l hc')
+    use Γ'
+    refine ⟨?_, hΓs⟩
+    constructor
+    · exact hτ₁
+    · exact weakening' h hΓs.left
+  | AppV v t₂ σ t₂' σ' hc₂ ih =>
+    obtain ⟨t₁, ht₁⟩ := v
+    obtain ⟨t₂, ht₂⟩ := t₂
+    cases hτ
+    expose_names
+    obtain ⟨Γ', ⟨hτ₂, hΓs⟩⟩ := ih (valid_app_r hc) h hσ hΓ (valid_app_r hc')
+    use Γ'
+    refine ⟨?_, hΓs⟩
+    constructor
+    · exact weakening' h_1 hΓs.left
+    · exact hτ₂
+  | Asgn x t σ t' σ' ht ih =>
+    obtain ⟨t, hₜ⟩ := t
+    cases hτ
+    expose_names
+    obtain ⟨Γ', ⟨hτ, hΓs⟩⟩ := ih (valid_asgn hc) h hσ hΓ (valid_asgn hc')
+    refine ⟨Γ', ⟨?_, hΓs⟩⟩
+    constructor
+    · apply (Γ.getVal_iff_getVal? _ _).mpr at h_1
+      apply (Γ'.getVal_iff_getVal? _ _).mp
+      have ⟨⟨hsub, hs⟩, _⟩ := hΓs
+      use hsub h_1.fst
+      rw [← hs h_1.fst, h_1.snd]
+    · exact hτ
+  | AsgnV x v σ =>
+    obtain ⟨v, hv⟩ := v
+    cases hτ
+    expose_names
+    refine ⟨Γ, ⟨h, ⟨Store.ext_le_refl, ⟨?_, ?_⟩⟩⟩⟩
+    · symm
+      simp [Store.dom, hσ]
+      have ⟨h', hs⟩ := (Γ.getVal_iff_getVal? _ _).mpr h_1
+      exact hσ ▸ h'
+    · simp [Store.getVal]
+      intro a ha
+      have ⟨h', hs⟩ := (Γ.getVal_iff_getVal? _ _).mpr h_1
+      split_ifs with hax
+      · simpa only [hax, hs]
+      · apply hΓ
 end Types
+
+#print axioms Types.preservation
